got correctness definition set up

hashedelgamal.ec
@@ -1,6 +1,6 @@
 (* Hashed el'gamal proof *)
 
-require import AllCore Distr.
+require import AllCore Distr SmtMap.
 
 type group.
 
@@ -18,13 +18,19 @@ axiom grpC (x y : group) : x ^^ y = y ^^ x.
 
 type exp.
 
-op (+*) : exp -> exp -> exp.
+op ( * ) : exp -> exp -> exp.
 
-axiom expA (x y z : exp) : x +* y +* z = x +* (y +* z).
+axiom expA (x y z : exp) : x * y * z = x * (y * z).
 
-axiom expC (x y : exp) : x +* y = y +* x.
+axiom expC (x y : exp) : x * y = y * x.
 
 op dexp : exp distr.
+
+axiom dexp_fu : is_full dexp.
+
+axiom dexp_uni : is_uniform dexp.
+
+axiom dexp_ll : is_lossless dexp.
 
 op g : group.
 
@@ -32,11 +38,26 @@ op (^) : group -> exp -> group.
 
   (* forall (x : group), unique (q : exp), s.t. x = g^q *)
 
-axiom uni : forall (x : group), exists (q : exp),  x = g ^ q.
+axiom generated (x : group) : exists (q : exp),  x = g ^ q.
 
-axiom grexpA (q1 q2 : exp) : (g ^ q1) ^ q2 = g ^ (q1 +* q2).
+axiom grexpA (q1 q2 : exp) : (g ^ q1) ^ q2 = g ^ (q1 * q2).
 
-lemma grexpAll (x : group) (q1 q2 : exp) : (x ^ q1) ^q2 = x ^ (q1 +* q2).
+op gen (q : exp) = g ^ q.
+axiom inj (q1 q2 : exp) : g^q1 = g^q2 => q1 = q2.
+
+op gen_rel (x : group)(q : exp) : bool = x = g^q.
+
+op log (x : group) : exp = choiceb (gen_rel x) e.
+
+lemma gen_log : cancel gen log.
+    proof.
+      rewrite /gen /log /cancel => q.
+    
+  qed.
+  
+
+
+lemma grexpAll (x : group) (q1 q2 : exp) : (x ^ q1) ^q2 = x ^ (q1 * q2).
     proof.
       admit. 
     
@@ -59,7 +80,41 @@ axiom textR (x : text) : x +^ x = text0.
 
 op dtext : text distr.
 
+axiom dtext_fu : is_full dtext.
 
+axiom dtext_uni : is_uniform dtext.
+
+axiom dtext_ll : is_lossless dtext.
+
+type cipher = group * text.
+
+(* Defining Correctness *)
+module type ENC = {
+  proc key_gen() : group * exp
+
+  proc enc(pubk : group, t : text) : cipher
+
+  proc dec(privk : exp, c : cipher) : text
+}.
+
+(* module to check for correctness of encryption scheme.
+
+    is correct if it the original input = final output when run through all funcitons with probability 1 *)
+
+module Cor (Enc : ENC) = {
+  proc main(x : text) : bool = {
+  var pubk : group; var privk : exp; var c : cipher; var y : text;
+    
+    (pubk, privk) <@ Enc.key_gen();
+      c <@ Enc.enc(pubk, x);
+      y <@ Enc.dec(privk, c);
+    return x = y;
+  }
+  
+}.
+
+
+(* concrete example of elgamal *)
       (* Random Oracle *)
 module type RO = {
   proc * init() : unit
@@ -69,10 +124,6 @@ module type RO = {
 
 module RO : RO = {
   var mp : (group, text) fmap (* finite map, table *)
-
-     x1 -> t1
-     x2 -> t2
-     x3 -> t3
 
   proc init() : unit = {
     mp <- empty;  (* empty map *)
@@ -86,39 +137,56 @@ module RO : RO = {
     }
     return oget mp.[x]; (* mp.[x] is either None or Some t *)
   }
-}
+}.
 
-module HEG (RO : RO) ={
-  proc key_gen() : exp = {
+
+module HEG (RO : RO) : ENC ={
+  proc key_gen() : group * exp = {
     var q : exp;
     q <$ dexp;
     return (g ^ q, q);
   }
 
-  proc enc(e : exp, t : text) : group {
-    var r : exp;
+  proc enc(pubk : group, t : text) : cipher = {
+      var r : exp;
+    var u : text;
     r <$ dexp;
     
-    (* Need to define pubk and privk. pubk = g ^ q and privk = q *)
-    u <@ RO.f(g ^ e ^ r);
+      (* Need to define pubk and privk. pubk = g ^ q and privk = q *)
+    u <@ RO.f(pubk ^ r);
 
     (*pubk ^ r = (g ^ q) ^ r = g ^ (q * r)*)
     return (g ^ r, t +^ u);
 
   }
 
-  proc dec(e : exp, g : group) : text {
-    u <@ RO.f(x ^ privk);
+  proc dec(privk : exp, c : cipher) : text = {
+    var u,v : text;
+      var x : group;
+
+    (x, u) <- c;
+    v <@ RO.f(x ^ privk);
     return v +^ u;
     (* (g ^ r) ^ q = g ^ (r * q) = g ^ (q * r) *)
     (*t +^ u +^ u = t =^ textO = t *)
   }
 
-}
+}.
 
 
+    (* prove encryption scheme is stateless *)
+
+lemma enc_stateless (g1 g2 : glob HEG) : g1 = g2.
+    proof.
+      trivial.
+  qed.
+
+      (* prove encryption scheme is correct *)
+lemma correctness : phoare[Cor(HEG).main : true ==> res] = 1%r.
+    proof.
+    
+  qed.
   
-
 
 
 
